completed the proof of undecidability for the fragement w/o unit

theories/BI/Utils/encoding.v
@@ -113,7 +113,16 @@ Section pseudo_exponential.
 
   Proof.
     rewrite <- Forall_forall in HΣ.
-    induction HΣ as [ | A Σ (γ & φ & ->) _ ]; simpl; eauto.
+    induction HΣ as [ | A Σ (γ & φ & ->) _ IH ] in Γ |- * ; simpl; eauto.
+    intros H.
+    apply LBI_equiv with (1 := BI_bequiv_sym (BI_bequiv_assoc _ _ _ _)),
+          LBI_equiv with (1 := BI_bequiv_comm _ _ _),
+          LBI_pseudo_exp_weak,
+          LBI_equiv with (1 := BI_bequiv_sym (BI_bequiv_assoc _ _ _ _)),
+          IH,
+          LBI_equiv with (1 := BI_bequiv_assoc _ _ _ _),
+          LBI_equiv with (1 := BI_bequiv_comm _ _ _).
+    revert H; apply LBI_equiv, BI_bequiv_assoc.
   Qed.
 
   (* We explain the "dereliction" rule as the combination of
@@ -137,12 +146,12 @@ Section pseudo_exponential.
 
   Local Proposition LBI_second_idea Γ γ φ :
 
-         (Γ ⊛ₘ ⟨(⊤-∗φ)⩑1⟩) ⊛ₐ ⟨φ⟩ ⊦ γ
+         (Γ ⊛ₘ ⟨(⊤-∗φ)⩑K⟩) ⊛ₐ ⟨φ⟩ ⊦ γ
     → (*------------------------------*)
-            Γ ⊛ₘ ⟨(⊤-∗φ)⩑1⟩ ⊦ γ.
+            Γ ⊛ₘ ⟨(⊤-∗φ)⩑K⟩ ⊦ γ.
 
   Proof.
-    set (Δ := Γ ⊛ₘ ⟨(⊤-∗φ)⩑1⟩).
+    set (Δ := Γ ⊛ₘ ⟨(⊤-∗φ)⩑K⟩).
     intros H.
     apply LBI_cntr_root.
     unfold Δ at 2.
@@ -172,18 +181,23 @@ Section pseudo_exponential.
   (* We generalize the dereliction rule to lists 
      containing a pseudo exponential ![γ]φ *)
 
-  Lemma LBI_list_mult_derilection Σ γ φ (HΣ : ![γ]φ ∊ Σ) :
+  Lemma LBI_list_mult_derilection Σ Γ γ φ (HΣ : ![γ]φ ∊ Σ) :
 
-        ⨂ₘ Σ ⊛ₘ ⟨φ⟩ ⊦ γ 
+        ⨂ₘ Σ ⊛ₘ ⟨φ⟩ ⊛ₘ Γ ⊦ γ 
     → (*---------------*)
-          ⨂ₘ Σ ⊦ γ.
+          ⨂ₘ Σ ⊛ₘ Γ ⊦ γ.
 
   Proof.
     revert HΣ; intros (Σ' & H'%BI_list_mult_perm_bequiv)%permutation_in_head H.
+    apply BI_bequiv_congr_r with (k := BI_mult) (Γ := Γ) in H'.
     apply LBI_equiv with (1 := BI_bequiv_sym H'); simpl.
-    apply LBI_equiv with (1 := BI_bequiv_comm _ _ _).
+    apply LBI_equiv with (1 := BI_bequiv_sym (BI_bequiv_assoc _ _ _ _)),
+          LBI_equiv with (1 := BI_bequiv_comm _ _ _).
     apply LBI_pseudo_exp_derilection.
     revert H; apply LBI_equiv.
+    apply BI_bequiv_trans with (1 := BI_bequiv_comm _ _ _),
+          BI_bequiv_trans with (1 := BI_bequiv_sym (BI_bequiv_assoc _ _ _ _)),
+          BI_bequiv_congr_r.
     do 2 apply BI_bequiv_sym,
                BI_bequiv_trans with (1 := BI_bequiv_comm _ _ _); eauto.
   Qed.
@@ -192,45 +206,50 @@ Section pseudo_exponential.
       (ie with FORK, INC, DEC and STOP but no zero test)
       in the (⩑,-∗) linear fragment of BI. *)
 
-  Local Fact LBI_FORK Γ φ ψ γ :
+  Local Fact LBI_FORK Γ Δ φ ψ γ :
 
-         Γ ⊦ φ    →    Γ ⊦ ψ 
-    → (*---------------------*)
-         Γ ⊛ₘ ⟨(φ⩑ψ)-∗γ⟩ ⊦ γ.
+         Γ ⊛ₘ Δ ⊦ φ    →    Γ ⊛ₘ Δ ⊦ ψ 
+    → (*-------------------------------*)
+           Γ ⊛ₘ ⟨(φ⩑ψ)-∗γ⟩ ⊛ₘ Δ ⊦ γ.
 
   Proof.
     intros.
-    apply LBI_impl_root; auto.
+    apply LBI_impl_middle; auto.
     now apply LBI_cntr_root, LBI_conj_r.
   Qed.
 
-  Local Fact LBI_INC Γ φ ψ γ :
+  Local Fact LBI_INC Γ Δ φ ψ γ :
 
-             Γ ⊛ₘ ⟨φ⟩ ⊦ ψ
+             Γ ⊛ₘ ⟨φ⟩ ⊛ₘ Δ ⊦ ψ
     → (*----------------------*)
-         Γ ⊛ₘ ⟨(φ-∗ψ)-∗γ⟩ ⊦ γ.
+         Γ ⊛ₘ ⟨(φ-∗ψ)-∗γ⟩ ⊛ₘ Δ ⊦ γ.
 
-  Proof. intros; apply LBI_impl_root; auto. Qed.
+  Proof.
+    intros; apply LBI_impl_middle; auto.
+    now apply LBI_impl_r, LBI_middle_move.
+  Qed.
 
-  Local Fact LBI_DEC Γ φ ψ γ :
+  Local Fact LBI_DEC Γ Δ φ ψ γ :
 
-                Γ ⊦ ψ
-    → (*---------------------------*)
-         Γ ⊛ₘ ⟨φ⟩ ⊛ₘ ⟨φ-∗ψ-∗γ⟩ ⊦ γ.
+                Γ ⊛ₘ Δ ⊦ ψ
+    → (*--------------------------------*)
+         Γ ⊛ₘ ⟨φ⟩ ⊛ₘ ⟨φ-∗ψ-∗γ⟩ ⊛ₘ Δ ⊦ γ.
 
   Proof.
     intros H.
-    apply LBI_equiv with (1 := BI_bequiv_sym (BI_bequiv_assoc _ _ _ _)).
-    rule LBI_impl_l at [rt].
-    apply LBI_impl_root; auto.
+    apply LBI_equiv with (Γ ⊛ₘ (⟨φ⟩ ⊛ₘ ⟨φ-∗ψ-∗γ⟩) ⊛ₘ Δ).
+    + apply BI_bequiv_congr_r, BI_bequiv_sym, BI_bequiv_assoc.
+    + apply LBI_middle_move.
+      rule LBI_impl_l at [rt].
+      apply LBI_impl_root; auto.
   Qed.
 
-  Local Fact LBI_STOP Γ γ :
-              Γ ⊦ 1
-    → (*-----------------*)
-         Γ ⊛ₘ ⟨1-∗γ⟩ ⊦ γ.
+  Local Fact LBI_STOP Γ Δ γ :
+              Γ ⊛ₘ Δ ⊦ K
+    → (*----------------------*)
+         Γ ⊛ₘ ⟨K-∗γ⟩ ⊛ₘ Δ ⊦ γ.
 
-  Proof. intros; apply LBI_impl_root; auto. Qed.
+  Proof. intros; apply LBI_impl_middle; auto. Qed.
 
   (* [Δ₁;...;Δₙ]--∗φ := Δ₁-∗...-∗Δₙ-∗φ *)
   Definition BI_multi_wand Δ (φ : BI_form µ prop) := fold_right (λ x y, x-∗y) φ Δ.
@@ -266,16 +285,18 @@ Section pseudo_exponential.
   Notation "⟦ A ⟧" := (tps_BI_form plus e s A).
 
   (* Semantically, ![γ]φ behaves much like φ⩑1 wrt TPS,
+     when K is interpreted the same way as 1
      hence irrelevant of the choice of γ *)
-  Proposition tps_BI_pseudo_exp γ φ : ⟦φ⟧ e → ∀x, ⟦![γ]φ⟧ x ↔ e = x.
+  Proposition tps_BI_pseudo_exp γ φ : (∀x, ⟦K⟧ x ↔ e = x) → ⟦φ⟧ e → ∀x, ⟦![γ]φ⟧ x ↔ e = x.
   Proof using comm neut.
-    intros Hφ x; split.
-    1: intros []; auto.
+    intros HK Hφ x; split.
+    1: intros []; apply HK; auto.
     intros <-.
-    split; [ | reflexivity ].
-    intros x _ H.
-    rewrite comm, neut in H.
-    rewrite comm; apply H; auto.
+    split; [ | ].
+    + intros x _ H.
+      rewrite comm, neut in H.
+      rewrite comm; apply H; auto.
+    + now apply HK.
   Qed. 
 
 End pseudo_exponential.
@@ -307,36 +328,41 @@ Section ACM2_to_BI.
   Variables (Σ : _) (l : _) (HΣl : ∀i, i ∊ Σ → src i ∊ l).
 
   (* Names for the two counters *)
+  
   Abbreviation α := true.
   Abbreviation β := false.
+  Abbreviation K := (£(inl (inr tt))).
+  Notation L x := (£(inl (inl x))).
 
   (** This is a "positive" encoding of 2-ACM in
       the (⩑,-∗) linear fragment of BI (ie IMLL)
         FORKₐ p q r --> q⩑r -∗ p
         INCₐ α p q  --> (α -∗ q) -∗ p
         DECₐ β p q  --> β -∗ q -∗ p
-        STOPₐ p     --> 1 -∗ p
+        STOPₐ p     --> K -∗ p
 
       Notice that locations in loc are encoded into
       variables in the left part of loc+bool
       while the right part is used from the two
       counters α/β *)
       
-  Definition acm2_instr_to_BI i : BI_form µ (loc+bool) :=
+  Definition acm2_instr_to_BI i : BI_form µ ((loc+unit)+bool) :=
     match i with
-    | FORKₐ p q r => (£(inl q) ⩑ £(inl r)) -∗ £(inl p)
-    | INCₐ c p q  => (£(inr c) -∗ £(inl q)) -∗ £(inl p)
-    | DECₐ c p q  => £(inr c) -∗ £(inl q) -∗ £(inl p)
-    | STOPₐ p     => 1 -∗ £(inl p)
+    | FORKₐ p q r => (L q ⩑ L r) -∗ L p
+    | INCₐ c p q  => (£(inr c) -∗ L q) -∗ L p
+    | DECₐ c p q  => £(inr c) -∗ L q -∗ L p
+    | STOPₐ p     => K -∗ L p
     end.
 
   Abbreviation encᵢ := acm2_instr_to_BI.
-  Notation "![ γ ] φ" := (BI_pseudo_exp γ φ).
+  Notation "![ γ ] φ" := (BI_pseudo_exp K γ φ).
+  
+  Definition acm2_code_to_BI := list_prod (λ p i, ![L p](encᵢ i)) l Σ.
 
   Definition acm2_ctx_to_BI x y :=
        repeat £(inr α) x
     ++ repeat £(inr β) y 
-    ++ list_prod (λ p i, ![£(inl p)](encᵢ i)) l Σ.
+    ++ acm2_code_to_BI.
 
   Abbreviation enc := acm2_ctx_to_BI.
 
@@ -346,7 +372,7 @@ Section ACM2_to_BI.
   Local Fact In_acm2_ctx_to_BI x y i p :
       i ∊ Σ 
     → p = src i
-    → ![£(inl p)](encᵢ i) ∊ enc x y.
+    → ![L p](encᵢ i) ∊ enc x y.
   Proof using HΣl.
     intros H1 H2.
     unfold acm2_ctx_to_BI.
@@ -378,14 +404,14 @@ Section ACM2_to_BI.
           Permutation_app_swap_app.
   Qed.
 
-  Hint Resolve In_acm2_ctx_to_BI : core.
+  Hint Resolve In_acm2_ctx_to_BI acm2_ctx_to_BI_x acm2_ctx_to_BI_y : core.
 
   Notation "Δ --∗ φ" := (BI_multi_wand Δ φ).
 
-  Definition acm2_to_BI x y p := 1⇒enc x y--∗£(inl p).
+  Definition acm2_to_BI x y p := ((map (λ _, K) acm2_code_to_BI)--∗K)⇒enc x y--∗(L p).
 
   (** We can now show that our positive encoding is sound
-      wrt to cut-free provability in the (-∗,⇒,⩑,1) fragment *)
+      wrt to cut-free provability in the (-∗,⇒,⩑) fragment *)
 
   Hint Constructors LBI_provable BI_bunch_equiv : core.
 
@@ -395,8 +421,9 @@ Section ACM2_to_BI.
   Proof using HΣl.
     intros H.
     apply LBI_impl_r, LBI_neut_l.
-    rule LBI_unit_l at [].
-    apply LBI_mult_wand_intro, LBI_neut_l.
+    (* rule LBI_unit_l at []. *)
+    apply LBI_mult_wand_intro,
+          LBI_equiv with (1 := BI_bequiv_comm _ _ _).
     revert H.
     induction 1 as [ p H 
                    | x y p q r H _ IH1 _ IH2
@@ -407,28 +434,31 @@ Section ACM2_to_BI.
                    ];
         match goal with
         | _ : ?i ∊ Σ |- _ => apply LBI_list_mult_derilection
-                               with (φ := acm2_instr_to_BI i)
+                               with (K := K) (φ := acm2_instr_to_BI i)
         end; auto; simpl acm2_instr_to_BI.
     + apply LBI_STOP.
-      unfold acm2_ctx_to_BI; simpl.
-      apply LBI_neut_r_inv with (k := BI_mult),
-            LBI_list_mult_weak; auto.
-      intros A (k & i & -> & [])%list_prod_spec; eauto.
+      unfold enc; simpl.
+      apply LBI_list_mult_weak with K.
+      1: intros A (k & i & -> & [])%list_prod_spec; eauto.
+      (* we show K^n ⊛ₘ (K^n --∗K) ⊦ K *)
+      induction acm2_code_to_BI as [ | ? m IH]; simpl.
+      * apply LBI_equiv with ⟨K⟩; auto.
+      * apply LBI_middle_move.
+        rule LBI_impl_l at [lft].
+        revert IH; apply LBI_equiv.
+        apply BI_bequiv_comm.
     + apply LBI_FORK; auto.
     + apply LBI_INC.
       revert IH; apply LBI_equiv; auto.
     + apply LBI_INC.
       revert IH; apply LBI_equiv; auto.
-      apply BI_bequiv_sym, 
-            BI_bequiv_trans with (1 := BI_list_mult_snoc _ _),
-            BI_list_mult_perm_bequiv.
-      unfold acm2_ctx_to_BI.
-      apply perm_trans with (2 := Permutation_app_swap_app _ _ _),
-            perm_skip,
-            Permutation_app_swap_app.
-    + apply LBI_equiv with (1 := BI_bequiv_sym (acm2_ctx_to_BI_x _ _ _)).
+    + apply LBI_equiv with (1 := BI_bequiv_sym (BI_bequiv_assoc _ _ _ _)),
+            LBI_equiv with (1 := BI_bequiv_sym (acm2_ctx_to_BI_x _ _ _)),
+            LBI_equiv with (1 := (BI_bequiv_assoc _ _ _ _)).
       now apply LBI_DEC.
-    + apply LBI_equiv with (1 := BI_bequiv_sym (acm2_ctx_to_BI_y _ _ _)).
+    + apply LBI_equiv with (1 := BI_bequiv_sym (BI_bequiv_assoc _ _ _ _)),
+            LBI_equiv with (1 := BI_bequiv_sym (acm2_ctx_to_BI_y _ _ _)),
+            LBI_equiv with (1 := (BI_bequiv_assoc _ _ _ _)).
       now apply LBI_DEC.
   Qed.
 
@@ -439,14 +469,21 @@ Section ACM2_to_BI.
         where (x,y) in nat² represents the value of
         α/β. *)
 
-    Local Definition tps (v : loc + bool) :=
+    Local Definition tps (v : loc + unit + bool) :=
       match v with
-      | inl p => λ '(x,y), acm2_accept Σ x y p
-      | inr α => eq (1,0)%nat 
-      | inr β => eq (0,1)%nat
+      | inl (inl p) => λ '(x,y), acm2_accept Σ x y p
+      | inl (inr _) => eq (0,0)%nat 
+      | inr α       => eq (1,0)%nat 
+      | inr β       => eq (0,1)%nat
       end.
 
     Notation "⟦ A ⟧" := (tps_BI_form pair_add (0,0) tps A).
+
+    Fact tps_map_K m : ⟦map (λ _ : BI_form µ (loc + unit + bool), K) m--∗K⟧ (0, 0).
+    Proof.
+      induction m; simpl; auto.
+      intros ? <-; simpl; auto.
+    Qed.
 
     Hint Constructors acm2_accept : core.
 
@@ -497,9 +534,10 @@ Section ACM2_to_BI.
 
     Lemma acm2_encode_complete : acm2_accept Σ x y p.
     Proof using Hxyp.
-      change (tps (inl p) (x,y)).
+      change (tps (inl (inl p)) (x,y)).
       simpl in Hxyp.
-      specialize (Hxyp eq_refl).
+      specialize (Hxyp _ (tps_map_K _)).
+      unfold tps_impl in Hxyp.
       unfold enc in Hxyp.
       rewrite !BI_mult_wand_app in Hxyp.
       apply tps_BI_multi_wand_α,
@@ -508,7 +546,8 @@ Section ACM2_to_BI.
       apply tps_BI_multi_wand_zero in Hxyp; auto.
       intros B (? & i & -> & [])%list_prod_spec.
       apply tps_BI_pseudo_exp; auto.
-      now apply tps_instr_sound.
+      + simpl; tauto. 
+      + now apply tps_instr_sound.
     Qed.
 
   End completeness.
@@ -523,8 +562,8 @@ Definition acm2_to_BI_form (loc : Set) Σ x y (p : loc) µ' Hµ' :=
   BI_form_map µ' Hµ' (λ x, x) (acm2_to_BI Σ (map acm2_instr_src Σ) x y p).
 
 (** This establishes the correctness of the reductions
-    2-ACM ⪯ LBI(-∗,⇒,⩑,1) ⪯ LBI ⪯ HBI(full) ⪯ 2-ACM 
-    where LBI is a fragment containing (-∗,⇒,⩑,1) and with
+    2-ACM ⪯ LBI(-∗,⇒,⩑) ⪯ LBI ⪯ HBI(full) ⪯ 2-ACM 
+    where LBI is a fragment containing (-∗,⇒,⩑) and with
     possibly the cut-rule *)
 Theorem acm2_to_BI_correctness (loc : Set) Σ x y (p : loc) µ' Hµ' cut :
     (acm2_accept Σ x y p → øₐ ⊦ acm2_to_BI Σ (map acm2_instr_src Σ) x y p)
